finish new FsLayout.v with proof
new FsLayout proves that its three partitions (inodes, bmaps, and blocks)
are disjoint.

with the help of the previously-proven RefineParts, this also means we
can stack anything on top of the individual partitions, and get the
compiler and proof of the entire FsLayout for free (as long as we
prove refinement for the particular thing we stack).

the proof is, at some level, pretty simple, but ends up long because
a slight detail differs for each of the 3 partitions, and i couldn't
figure out how to automate the "instantiate" tactic.

src/DiskMod.v
@@ -25,8 +25,8 @@ Definition eq_addr_dec (a b:addr) : {a=b}+{a<>b}.
 Defined.
 
 Inductive prog {R:Type} : Type :=
-  | Read (b:addr) (rx:block->prog)
-  | Write (b:addr) (v:block) (rx:unit->prog)
+  | Read (a:addr) (rx:block->prog)
+  | Write (a:addr) (v:block) (rx:unit->prog)
   | Return (v:R).
 Definition Prog := @prog.
 Definition ReturnOp := @Return.
@@ -34,12 +34,12 @@ Definition State := addr -> block.
 
 Inductive step {R:Type} : @progstate R Prog State ->
                           @progstate R Prog State -> Prop :=
-  | StepRead: forall d b rx,
-    step (PS (Read b rx) d)
-         (PS (rx (d b)) d)
-  | StepWrite: forall d b v rx,
-    step (PS (Write b v rx) d)
-         (PS (rx tt) (setidx eq_addr_dec d b v)).
+  | StepRead: forall d a rx,
+    step (PS (Read a rx) d)
+         (PS (rx (d a)) d)
+  | StepWrite: forall d a v rx,
+    step (PS (Write a v rx) d)
+         (PS (rx tt) (setidx eq_addr_dec d a v)).
 Definition Step := @step.
 
 Theorem opp_step_wf:
